fix: wfty

CollapsingTowers/TwoLevel/Basic.lean
@@ -11,15 +11,16 @@ def wfty₁ : Ty -> Prop
   | .arrow τ𝕒 τ𝕓 => wfty₁ τ𝕒 /\ wfty₁ τ𝕓
   | .rep _ => false
 
-@[simp]
-def wfty₂ : Ty -> Prop
-  | .nat => false
-  | .arrow τ𝕒 τ𝕓 => wfty₂ τ𝕒 \/ wfty₂ τ𝕓
-  | .rep τ => wfty₁ τ
-
-@[simp]
-def wfty (τ : Ty) : Prop :=
-  wfty₁ τ \/ wfty₂ τ
+mutual
+  @[simp]
+  def wfty₂ : Ty -> Prop
+    | .nat => false
+    | .arrow τ𝕒 τ𝕓 => (wfty₂ τ𝕒 /\ wfty τ𝕓) \/ (wfty τ𝕒 /\ wfty₂ τ𝕓)
+    | .rep τ => wfty₁ τ
+  @[simp]
+  def wfty (τ : Ty) : Prop :=
+    wfty₁ τ \/ wfty₂ τ
+end
 
 inductive Expr : Type where
   | bvar (i : ℕ)
